\documentclass[12pt]{article}
\usepackage{bussproofs}
\usepackage{listings}
\usepackage{amssymb}
\usepackage[total={10in, 7in}, top=0.5in, bottom=0.5in, left=0.5in, right=0.5in, landscape]{geometry}

\renewcommand{\familydefault}{\sfdefault}
\begin{document}
  \begin{lstlisting}
    { true }
    z = 0;
    sum = 0;
    while i != x
      i := i + 1;
      sum := sum + y;
    { sum = x * y }
  \end{lstlisting}

  Let $w$ be the while loop.

  \section{Question 1}
  Using Hoare's rules, prove:
  $$\{x = y\} x:= x+1; y:=y+1 \{x = y\}$$
  \subsection{Answer}
  Here all the rules belong to Hoare's rules for While. So, ignored the $\vdash$ in the triples.
  \begin{prooftree}
            \AxiomC{$x = y \Rightarrow true $}
                \AxiomC{$\{x+1 = y +1\} x:= x+1 \{x = y + 1\} $}
                \RightLabel{\scriptsize($ass_t$ rule)}
            \UnaryInfC{$\{true\} x:= x+1 \{x = y +1\} $}
            \RightLabel{\scriptsize($cons_t$)}
        \BinaryInfC{$\{x = y\} x:= x+1 \{x = y +1\} $}
            \RightLabel{\scriptsize($ass_t$)}
            \AxiomC{$ \{[y+1/y](x=y)\} y:=y+1 \{x = y\} $}
        \UnaryInfC{$ \{x = y +1\} y:=y+1 \{x = y\} $}
        \RightLabel{\scriptsize( $comp_t$ )}
    \BinaryInfC{$\{x = y\} x:= x+1; y:=y+1 \{x = y\}$}
  \end{prooftree}

  \section{Question 2}
  Using Hoareâ€™s rules, prove
  $$ \{ y = z \}  \textrm{ while b do } y := y - x \{ \exists k. z = (y + k * x)\} $$
  for an arbitrary boolean expression b.
  \subsection{Answer}
  Let's define W = $\textrm{ while b do } y := y - x $ \\
  First we need to find the lopp invariant I so that we can apply the while rule. In this case the invariant is $x = n$ \\
  Loop invariant: $\exists j\exists k. y = z - j*x \wedge k = j + 1$ \\


  \begin{prooftree}
        \AxiomC{$y = z \Rightarrow \exists j\exists k. y = z - j*x \wedge k = j + 1$}
            \AxiomC{${D1:}\{ \exists j\exists k. y = z - j*x \wedge k = j + 1 \wedge b\} y:=y-x \{ \exists j \exists k. y = z - (j+1)*x  \wedge k = j + 1 \}  $}
        \UnaryInfC{$\{ \exists j\exists k. y = z - j*x \wedge k = j + 1 \} W \{ \exists j \exists k. y = z - (j+1)*x  \wedge k = j + 1 \wedge \neg b \}  $}
    \BinaryInfC{$\{ y = z \} \textrm{ while b do } y := y - x \{ \exists k. z = (y + k * x)\} $}
      
  \end{prooftree}
  \begin{prooftree}
    \AxiomC{$\exists j\exists k. y = z - j*x \wedge k = j + 1 \wedge b \Rightarrow true$}
        \AxiomC{$\{ true \} y:=y-x \{ \exists j \exists k. y = z - (j+1)*x  \wedge k = j + 1 \}  $}
        \LeftLabel{D1:}
    \BinaryInfC{$\{ \exists j\exists k. y = z - j*x \wedge k = j + 1 \wedge b\} y:=y-x \{ \exists j \exists k. y = z - (j+1)*x  \wedge k = j + 1 \}  $}
    
      
  \end{prooftree}



\end{document}